Changed ZXperm back to being definitionally ZX n n, and significantly overhauled permutations automation to make this (casting) bearable. Updated the category-theoretic proofs that use it.

src/Permutations/PermutationFacts.v
@@ -55,8 +55,18 @@ Lemma perm_inv_bdd_S n f k :
   perm_inv (S n) f k < S n.
 Proof.
   induction n; simpl;
+<<<<<<< Updated upstream
+<<<<<<< Updated upstream
+  [bdestructΩ'|]. 
+  bdestruct_one; [|transitivity (S n); [apply IHn|]]. 
+=======
   [destruct_if_solve|]. 
   destruct_if; [|transitivity (S n); [apply IHn|]]. 
+>>>>>>> Stashed changes
+=======
+  [destruct_if_solve|]. 
+  destruct_if; [|transitivity (S n); [apply IHn|]]. 
+>>>>>>> Stashed changes
   all: apply Nat.lt_succ_diag_r.
 Qed.
 
@@ -139,6 +149,19 @@ Proof.
     apply Hsurj; easy.
 Qed.
 
+<<<<<<< Updated upstream
+<<<<<<< Updated upstream
+
+Local Notation perm_surj n f := (forall k, k < n -> exists k', k' < n /\ f k' = k).
+Local Notation perm_bdd  n f := (forall k, k < n -> f k < n).
+Local Notation perm_inj  n f := (forall k l, k < n -> l < n -> f k = f l -> k = l).
+(* Local Notation WF_perm   n f := (forall k, n <= k -> f k = k). *)
+
+
+(* FIXME: In QuantumLib *)
+=======
+=======
+>>>>>>> Stashed changes
 (* FIXME: Should these exist? *)
 Local Notation perm_surj n f := (forall k, k < n -> exists k', k' < n /\ f k' = k).
 Local Notation perm_bdd  n f := (forall k, k < n -> f k < n).
@@ -146,7 +169,29 @@ Local Notation perm_inj  n f := (forall k l, k < n -> l < n -> f k = f l -> k = 
 Local Notation perm_WF   n f := (forall k, n <= k -> f k = k).
 
 
+(* TODO: Move this where it belongs *)
+<<<<<<< Updated upstream
+>>>>>>> Stashed changes
+=======
+>>>>>>> Stashed changes
+Lemma fswap_involutive : forall {A} (f : nat -> A) x y,
+  fswap (fswap f x y) x y = f.
+Proof.
+  intros A f x y.
+  unfold fswap.
+  apply functional_extensionality.
+  intros k.
+  bdestruct_all; subst; easy.
+Qed.
 
+<<<<<<< Updated upstream
+<<<<<<< Updated upstream
+
+
+=======
+>>>>>>> Stashed changes
+=======
+>>>>>>> Stashed changes
 Lemma fswap_injective_if_injective : forall {A} n (f:nat -> A) x y,
   x < n -> y < n ->
   perm_inj n f -> perm_inj n (fswap f x y).
@@ -285,7 +330,15 @@ Proof.
   apply Hinj; auto; lia.
 Qed.
 
+<<<<<<< Updated upstream
+<<<<<<< Updated upstream
 Lemma injective_and_bounded_grow_of_boundary : forall n f,
+=======
+Lemma injective_and_bdd_grow_of_boundary : forall n f,
+>>>>>>> Stashed changes
+=======
+Lemma injective_and_bdd_grow_of_boundary : forall n f,
+>>>>>>> Stashed changes
   perm_inj n f /\ perm_bdd n f -> f n = n ->
   perm_inj (S n) f /\ perm_bdd (S n) f.
 Proof.
@@ -311,7 +364,15 @@ Proof.
       lia.
 Qed.
 
+<<<<<<< Updated upstream
+<<<<<<< Updated upstream
 Lemma injective_and_bounded_of_surjective : forall n f,
+=======
+Lemma injective_and_bdd_of_surjective : forall n f,
+>>>>>>> Stashed changes
+=======
+Lemma injective_and_bdd_of_surjective : forall n f,
+>>>>>>> Stashed changes
   perm_surj n f -> perm_inj n f /\ perm_bdd n f.
 Proof.
   intros n.
@@ -323,12 +384,28 @@ Proof.
   specialize (IHn (fswap f n' n) Hswap_surj).
   rewrite (fswap_injective_iff_injective _ f n' n); [|easy|easy].
   rewrite (fswap_bounded_iff_bounded _ f n' n); [|easy|easy].
+<<<<<<< Updated upstream
+<<<<<<< Updated upstream
   apply injective_and_bounded_grow_of_boundary;
+=======
+  apply injective_and_bdd_grow_of_boundary;
+>>>>>>> Stashed changes
+=======
+  apply injective_and_bdd_grow_of_boundary;
+>>>>>>> Stashed changes
   [| rewrite fswap_simpl2; easy].
   easy.
 Qed.
 
+<<<<<<< Updated upstream
+<<<<<<< Updated upstream
 Lemma injective_and_bounded_shrink_of_boundary : forall n f,
+=======
+Lemma injective_and_bdd_shrink_of_boundary : forall n f,
+>>>>>>> Stashed changes
+=======
+Lemma injective_and_bdd_shrink_of_boundary : forall n f,
+>>>>>>> Stashed changes
   perm_inj (S n) f /\ perm_bdd (S n) f -> f n = n -> 
   perm_inj n f /\ perm_bdd n f.
 Proof.
@@ -346,6 +423,8 @@ Proof.
     + lia.
 Qed.
 
+<<<<<<< Updated upstream
+<<<<<<< Updated upstream
 (* Formalization of proof sketch of pigeonhole principle
    from https://math.stackexchange.com/a/910790 *)
 Lemma exists_bounded_decidable : forall n P,
@@ -437,11 +516,11 @@ Proof.
   (* Now, contradict injectivity using pigeonhole principle *)
   exfalso.
   assert (Hbdd': forall j, j < S n -> f j < n). 1:{
-  - intros j Hj.
+    intros j Hj.
     specialize (Hbdd j Hj).
     bdestruct (f j =? n).
-    + exfalso; apply Hnex; exists j; easy.
-    + lia.
+    - exfalso; apply Hnex; exists j; easy.
+    - lia.
   }
   destruct (pigeonhole_S n f Hbdd') as [i [j [Hi [Hj Heq]]]].
   absurd (i = j).
@@ -478,25 +557,117 @@ Qed.
 
 
 
+(* Section on WF_perm *)
+Lemma monotonic_WF_perm n m f : WF_perm n f -> n <= m ->
+  WF_perm m f.
+=======
+=======
+>>>>>>> Stashed changes
+Lemma surjective_of_inj_and_bdd : forall n f,
+  perm_inj n f /\ perm_bdd n f -> perm_surj n f.
+Proof.
+  induction n; [easy|].
+  intros f [Hinj Hbdd].
+  rewrite (fswap_surjective_iff_surjective _ _ n (perm_inv (S n) f n));
+  [|lia|apply perm_inv_bdd_S].
+  rewrite (fswap_injective_iff_injective _ _ n (perm_inv (S n) f n)) in Hinj;
+  [|lia|apply perm_inv_bdd_S].
+  rewrite (fswap_bounded_iff_bounded _ _ n (perm_inv (S n) f n)) in Hbdd;
+  [|lia|apply perm_inv_bdd_S].
+  assert (perm_surj n (fswap f n (perm_inv (S n) f n))).
+  1 : {
+    apply IHn, injective_and_bdd_shrink_of_boundary; [easy|].
+    rewrite fswap_simpl1.
+    admit.
+  }
+  apply surjective_of_eq_boundary_grow; [easy|].
+  Admitted.
+
+
+
+
+
+
+(* Lemma perm_inv_surj_of_surj n f :
+  (forall k, k < n -> exists l, l < n /\ f l = k) ->
+  forall l, l < n -> exists k, k < n /\ perm_inv n f k = l. *)
+
+
+
+
+
+(* Section for prelude lemmas that don't directly involve permutations *)
+(* TODO: Prove these: *)
+
+
+
+
+Lemma bdd_of_is_inj_is_surj n f :
+  perm_inj n f -> perm_surj n f -> perm_bdd n f.
+Proof.
+  intros Hinj Hsurj k Hk.
+
+  Abort.
+
+Lemma surj_of_is_bdd_is_inj n f : 
+  perm_bdd n f -> perm_inj n f -> perm_surj n f.
+Proof.
+  Abort.
+
+Lemma inj_of_is_surj_is_bdd n f :
+  perm_surj n f -> perm_bdd n f -> perm_inj n f. 
+Proof.
+  Abort. 
+
+(* Lemma surj_of_is_WF_is_inj n f *)
+
+
+
+
 (* Section on perm_WF *)
 Lemma monotonic_perm_WF n m f : perm_WF n f -> n <= m ->
   perm_WF m f.
+<<<<<<< Updated upstream
+>>>>>>> Stashed changes
+=======
+>>>>>>> Stashed changes
 Proof.
   intros HWF Hnm k Hk.
   apply HWF; lia.
 Qed.
 
+<<<<<<< Updated upstream
+<<<<<<< Updated upstream
+Global Hint Resolve monotonic_WF_perm : WF_perm_db.
+
+Lemma compose_WF_perm n f g : WF_perm n f -> WF_perm n g -> 
+  WF_perm n (f ∘ g).
+=======
+=======
+>>>>>>> Stashed changes
 Global Hint Resolve monotonic_perm_WF : perm_WF_db.
 
 Lemma compose_perm_WF n f g : perm_WF n f -> perm_WF n g -> 
   perm_WF n (f ∘ g).
+<<<<<<< Updated upstream
+>>>>>>> Stashed changes
+=======
+>>>>>>> Stashed changes
 Proof.
   unfold compose.
   intros Hf Hg k Hk.
   rewrite Hg, Hf; easy.
 Qed.
 
+<<<<<<< Updated upstream
+<<<<<<< Updated upstream
+Global Hint Resolve compose_WF_perm : WF_perm_db.
+=======
 Global Hint Resolve compose_perm_WF : perm_WF_db.
+>>>>>>> Stashed changes
+=======
+Global Hint Resolve compose_perm_WF : perm_WF_db.
+>>>>>>> Stashed changes
 
 Lemma linv_WF_of_WF {n} {f finv}
 	(HfWF : forall k, n <= k -> f k = k) (Hinv : finv ∘ f = idn) :
@@ -553,30 +724,97 @@ Qed.
 
 
 Lemma permutation_of_le_permutation_WF f m n : (m <= n)%nat -> permutation m f ->
-  perm_WF m f -> permutation n f.
+  WF_perm m f -> permutation n f.
 Proof.
   intros Hmn [finv_m Hfinv_m] HWF.
   exists (fun k => if m <=? k then k else finv_m k).
   intros k Hk.
   bdestruct (m <=? k).
-  - rewrite HWF; destruct_if_solve.
+  - rewrite HWF; bdestructΩ'.
   - specialize (Hfinv_m _ H).
-    repeat split; destruct_if_solve.
+    bdestructΩ'.
 Qed.
 
+<<<<<<< Updated upstream
 (* FIXME: ^ All this is now in QuantumLib*)
 
 
 (* FIXME: TODO: This is *really* not where this goes! But right now, it needs to. *)
-Ltac by_inverse_injective f n :=
+(* Once quantumlib's in, we can put this in automation directly. *)
+Ltac perm_eq_by_WF_inv_inj f n :=
+  let tryeasylia := try easy; try lia in 
   apply (WF_permutation_inverse_injective f n); [
     tryeasylia; auto with perm_db |
-    tryeasylia; auto with perm_WF_db |
+    tryeasylia; auto with WF_perm_db |
     try solve [cleanup_perm; auto] |
     try solve [cleanup_perm; auto]]; tryeasylia.
 
 
 
+
+
+
+
+
+
+
+
+
+
+
+
+
+
+
+
+(* TODO FIXME: Should this really be here? *)
+(* Section on swap_perm, swaps two elements. TODO: Do we even want this?
+	 We have swap_2_perm and fswap... Also, should swap_perm be defined in 
+	 terms of fswap? *)
+Lemma swap_perm_same a n :
+  swap_perm a a n = idn.
+Proof.
+  unfold swap_perm.
+  apply functional_extensionality; intros k.
+  bdestructΩ'.
+Qed.
+
+#[export] Hint Rewrite swap_perm_same : perm_cleanup_db.
+
+Lemma swap_perm_comm a b n :
+  swap_perm a b n = swap_perm b a n.
+Proof.
+  apply functional_extensionality; intros k.
+  unfold swap_perm.
+  bdestructΩ'.
+Qed.
+
+Lemma swap_WF_perm a b n : forall k, n <= k -> swap_perm a b n k = k.
+Proof.
+  intros.
+  unfold swap_perm. 
+  bdestructΩ'.
+Qed.
+
+Global Hint Resolve swap_WF_perm : WF_perm_db.
+
+Lemma swap_perm_bdd a b n : a < n -> b < n ->
+  forall k, k < n -> swap_perm a b n k < n.
+Proof.
+  intros Ha Hb k Hk.
+  unfold swap_perm.
+  bdestructΩ'.
+Qed.
+
+<<<<<<< Updated upstream
+Global Hint Resolve swap_perm_bdd : perm_bdd_db.
+
+Lemma swap_perm_inv a b n : a < n -> b < n -> 
+  (swap_perm a b n) ∘ (swap_perm a b n) = idn.
+Proof.
+=======
+=======
+>>>>>>> Stashed changes
 
 
 
@@ -627,6 +865,7 @@ Global Hint Resolve swap_perm_WF : perm_WF_db.
 
 Lemma swap_perm_bdd a b n : a < n -> b < n ->
   forall k, k < n -> swap_perm a b n k < n.
+<<<<<<< Updated upstream
 Proof.
   intros Ha Hb k Hk.
   unfold swap_perm.
@@ -638,11 +877,33 @@ Global Hint Resolve swap_perm_bdd : perm_bdd_db.
 Lemma swap_perm_inv a b n : a < n -> b < n -> 
   (swap_perm a b n) ∘ (swap_perm a b n) = idn.
 Proof.
+>>>>>>> Stashed changes
+=======
+Proof.
+  intros Ha Hb k Hk.
+  unfold swap_perm.
+  destruct_if_solve.
+Qed.
+
+Global Hint Resolve swap_perm_bdd : perm_bdd_db.
+
+Lemma swap_perm_inv a b n : a < n -> b < n -> 
+  (swap_perm a b n) ∘ (swap_perm a b n) = idn.
+Proof.
+>>>>>>> Stashed changes
   intros Ha Hb.
   unfold compose.
   apply functional_extensionality; intros k.
   unfold swap_perm.
+<<<<<<< Updated upstream
+<<<<<<< Updated upstream
+  bdestructΩ'.
+=======
   destruct_if_solve.
+>>>>>>> Stashed changes
+=======
+  destruct_if_solve.
+>>>>>>> Stashed changes
 Qed.
 
 #[export] Hint Rewrite swap_perm_inv : perm_inv_db.
@@ -671,7 +932,15 @@ Proof.
   intros Ha Hb Hc Hbc Hac. 
   apply functional_extensionality; intros k.
   unfold compose, swap_perm.
+<<<<<<< Updated upstream
+<<<<<<< Updated upstream
+  bdestructΩ'.
+=======
   destruct_if_solve.
+>>>>>>> Stashed changes
+=======
+  destruct_if_solve.
+>>>>>>> Stashed changes
 Qed.
 
 #[export] Hint Rewrite compose_swap_perm : perm_cleanup_db.
@@ -689,6 +958,74 @@ Proof.
   apply functional_extensionality; intros k.
   unfold compose, fswap, swap_perm.
   bdestruct_all; easy.
+<<<<<<< Updated upstream
+Qed.
+
+Lemma fswap_perm_inv_n_permutation f n : permutation (S n) f ->
+  permutation n (fswap f (perm_inv (S n) f n) n).
+Proof.
+  intros Hperm.
+  apply fswap_at_boundary_permutation.
+  - apply Hperm.
+  - apply perm_inv_bdd_S.
+  - apply perm_inv_is_rinv_of_permutation; auto.
+Qed.
+
+(* Notation perm_list_of_insertion_sort_list l :=
+  (map (fun idxk => match idxk with 
+    | pair n k => swap_perm n k (S n)
+    end) (combine (seq 0 (length l)) l)). *)
+
+Fixpoint swap_list_spec l : bool :=
+  match l with 
+  | [] => true
+  | k :: ks => (k <? S (length ks)) && swap_list_spec ks
+  end.
+
+Fixpoint perm_of_swap_list l :=
+  match l with
+  | [] => idn
+  | k :: ks => let n := length ks in
+    (swap_perm k n (S n) ∘ (perm_of_swap_list ks))
+  end.
+
+Fixpoint invperm_of_swap_list l :=
+  match l with 
+  | [] => idn
+  | k :: ks => let n := length ks in
+    ((invperm_of_swap_list ks) ∘ swap_perm k n (S n))
+  end.
+
+Local Opaque perm_inv.
+Lemma perm_of_swap_list_WF l : swap_list_spec l = true ->
+<<<<<<< Updated upstream
+  WF_perm (length l) (perm_of_swap_list l).
+=======
+  perm_WF (length l) (perm_of_swap_list l).
+>>>>>>> Stashed changes
+Proof.
+  induction l.
+  - easy.
+  - simpl.
+    rewrite andb_true_iff.
+    intros [Ha Hl].
+    intros k Hk.
+    unfold compose.
+    rewrite IHl; [|easy|lia].
+<<<<<<< Updated upstream
+    rewrite swap_WF_perm; easy.
+Qed.
+
+Lemma invperm_of_swap_list_WF l : swap_list_spec l = true ->
+  WF_perm (length l) (invperm_of_swap_list l).
+=======
+    rewrite swap_perm_WF; easy.
+Qed.
+
+Lemma invperm_of_swap_list_WF l : swap_list_spec l = true ->
+  perm_WF (length l) (invperm_of_swap_list l).
+>>>>>>> Stashed changes
+=======
 Qed.
 
 Lemma fswap_perm_inv_n_permutation f n : permutation (S n) f ->
@@ -729,6 +1066,7 @@ Fixpoint invperm_of_swap_list l :=
 Local Opaque perm_inv.
 Lemma perm_of_swap_list_WF l : swap_list_spec l = true ->
   perm_WF (length l) (perm_of_swap_list l).
+>>>>>>> Stashed changes
 Proof.
   induction l.
   - easy.
@@ -737,6 +1075,40 @@ Proof.
     intros [Ha Hl].
     intros k Hk.
     unfold compose.
+<<<<<<< Updated upstream
+<<<<<<< Updated upstream
+    rewrite swap_WF_perm; [|easy].
+    rewrite IHl; [easy|easy|lia].
+Qed.
+
+Global Hint Resolve perm_of_swap_list_WF invperm_of_swap_list_WF : WF_perm_db.
+=======
+    rewrite swap_perm_WF; [|easy].
+    rewrite IHl; [easy|easy|lia].
+Qed.
+
+Global Hint Resolve perm_of_swap_list_WF invperm_of_swap_list_WF : perm_WF_db.
+>>>>>>> Stashed changes
+
+Lemma invperm_linv_perm_of_swap_list l : swap_list_spec l = true ->
+  invperm_of_swap_list l ∘ perm_of_swap_list l = idn.
+Proof.
+  induction l.
+  - easy.
+  - simpl. 
+    rewrite andb_true_iff.
+    intros [Ha Hl].
+    rewrite Combinators.compose_assoc, 
+    <- (Combinators.compose_assoc _ _ _ _ (perm_of_swap_list _)).
+    rewrite swap_perm_inv, compose_idn_l.
+    + apply (IHl Hl).
+    + bdestructΩ (a <? S (length l)).
+    + lia.
+Qed.
+
+Lemma invperm_rinv_perm_of_swap_list l : swap_list_spec l = true ->
+  perm_of_swap_list l ∘ invperm_of_swap_list l = idn.
+=======
     rewrite IHl; [|easy|lia].
     rewrite swap_perm_WF; easy.
 Qed.
@@ -759,12 +1131,48 @@ Global Hint Resolve perm_of_swap_list_WF invperm_of_swap_list_WF : perm_WF_db.
 
 Lemma invperm_linv_perm_of_swap_list l : swap_list_spec l = true ->
   invperm_of_swap_list l ∘ perm_of_swap_list l = idn.
+>>>>>>> Stashed changes
 Proof.
   induction l.
   - easy.
   - simpl. 
     rewrite andb_true_iff.
     intros [Ha Hl].
+<<<<<<< Updated upstream
+    rewrite <- Combinators.compose_assoc,
+    (Combinators.compose_assoc _ _ _ _ (invperm_of_swap_list _)).
+    rewrite (IHl Hl).
+    rewrite compose_idn_r.
+    rewrite swap_perm_inv; [easy| |lia].
+    bdestructΩ (a <? S (length l)).
+Qed.
+
+#[export] Hint Rewrite invperm_linv_perm_of_swap_list 
+  invperm_rinv_perm_of_swap_list : perm_cleanup_db.
+
+
+(* FIXME: Remove; for working reference*)
+Fixpoint insertion_sort_list n f := 
+  match n with 
+  | 0 => []
+  | S n' => let k := (perm_inv (S n') f n') in
+      k :: insertion_sort_list n' (fswap f k n')
+  end.
+
+Lemma length_insertion_sort_list n f :
+  length (insertion_sort_list n f) = n.
+Proof.
+  revert f;
+  induction n;
+  intros f.
+  - easy.
+  - simpl.
+    rewrite IHn; easy.
+Qed.
+
+Lemma insertion_sort_list_is_swap_list n f : 
+  swap_list_spec (insertion_sort_list n f) = true.
+=======
     rewrite Combinators.compose_assoc, 
     <- (Combinators.compose_assoc _ _ _ _ (perm_of_swap_list _)).
     rewrite swap_perm_inv, compose_idn_l.
@@ -803,12 +1211,15 @@ Fixpoint insertion_sort_list n f :=
 
 Lemma length_insertion_sort_list n f :
   length (insertion_sort_list n f) = n.
+>>>>>>> Stashed changes
 Proof.
   revert f;
   induction n;
   intros f.
   - easy.
   - simpl.
+<<<<<<< Updated upstream
+=======
     rewrite IHn; easy.
 Qed.
 
@@ -820,6 +1231,7 @@ Proof.
   intros f.
   - easy.
   - simpl.
+>>>>>>> Stashed changes
     rewrite length_insertion_sort_list, IHn.
     pose proof (perm_inv_bdd_S n f n).
     bdestructΩ (perm_inv (S n) f n <? S n).
@@ -868,7 +1280,7 @@ Lemma stack_perms_left {n0 n1} {f g} {k} :
 Proof.
   intros Hk.
   unfold stack_perms.
-  bdest_lia_replace (k <? n0) true.
+  replace_bool_lia (k <? n0) true.
   easy.
 Qed.
 
@@ -877,8 +1289,8 @@ Lemma stack_perms_right {n0 n1} {f g} {k} :
 Proof.
   intros Hk.
   unfold stack_perms.
-  bdest_lia_replace (k <? n0) false.
-  bdest_lia_replace (k <? n0 + n1) true.
+  replace_bool_lia (k <? n0) false.
+  replace_bool_lia (k <? n0 + n1) true.
   easy.
 Qed.
 
@@ -903,23 +1315,23 @@ Lemma stack_perms_high {n0 n1} {f g} {k} :
 Proof.
 	intros H.
 	unfold stack_perms.
-	bdest_lia_replace (k <? n0) false. 
-	bdest_lia_replace (k <? n0 + n1) false.
+	replace_bool_lia (k <? n0) false. 
+	replace_bool_lia (k <? n0 + n1) false.
 	easy.
 Qed.
 
 Lemma stack_perms_f_idn n0 n1 f :
 	stack_perms n0 n1 f idn = fun k => if k <? n0 then f k else k.
-Proof. solve_stack_perm n0 n1. Qed. 
+Proof. solve_modular_permutation_equalities. Qed. 
 
 Lemma stack_perms_idn_f n0 n1 f : 
 	stack_perms n0 n1 idn f = 
 	fun k => if (¬ k <? n0) && (k <? n0 + n1) then f (k - n0) + n0 else k.
-Proof. solve_stack_perm n0 n1. Qed. 
+Proof. solve_modular_permutation_equalities. Qed. 
 
 Lemma stack_perms_idn_idn n0 n1 :
 	stack_perms n0 n1 idn idn = idn.
-Proof. solve_stack_perm n0 n1. Qed.
+Proof. solve_modular_permutation_equalities. Qed.
 
 #[export] Hint Rewrite stack_perms_idn_idn : perm_cleanup_db.
 
@@ -931,8 +1343,8 @@ Proof.
 	destruct Hf' as [Hf'inv Hf'].
 	destruct Hg' as [Hg'inv Hg'].
 	unfold compose.
-	(* destruct_if. *)
-	solve_stack_perm_strong n0 n1.
+	(* bdestruct_one. *)
+  solve_modular_permutation_equalities.
 	1,2: specialize (Hf' k H); lia.
 	- f_equal; f_equal. lia.
 	- assert (Hk: k - n0 < n1) by lia.
@@ -945,7 +1357,7 @@ Lemma stack_perms_assoc {n0 n1 n2} {f g h} :
 Proof.
   apply functional_extensionality; intros k.
   unfold stack_perms.
-  destruct_if_solve.
+  bdestructΩ'.
   rewrite (Nat.add_comm n0 n1), Nat.add_assoc.
   f_equal; f_equal; f_equal.
   lia.
@@ -955,7 +1367,7 @@ Lemma stack_perms_idn_of_left_right_idn {n0 n1} {f g}
   (Hf : forall k, k < n0 -> f k = k) (Hg : forall k, k < n1 -> g k = k) :
   stack_perms n0 n1 f g = idn.
 Proof.
-  solve_stack_perm n0 n1.
+  solve_modular_permutation_equalities.
   - apply Hf; easy.
   - rewrite Hg; lia.
 Qed.
@@ -970,25 +1382,25 @@ Qed.
 (* FIXME: Decide whether/how to put this back where it goes in PermutationInstances *)
 Lemma rotr_WF {n m} : 
 	forall k, n <= k -> (rotr n m) k = k.
-Proof. intros. unfold rotr. destruct_if; lia. Qed.
+Proof. intros. unfold rotr. bdestruct_one; lia. Qed.
 
 Lemma rotl_WF {n m} : 
 	forall k, n <= k -> (rotl n m) k = k.
-Proof. intros. unfold rotl. destruct_if; lia. Qed.
+Proof. intros. unfold rotl. bdestruct_one; lia. Qed.
 
-Global Hint Resolve rotr_WF rotl_WF : perm_WF_db.
+Global Hint Resolve rotr_WF rotl_WF : WF_perm_db.
 
 Lemma rotr_bdd {n m} : 
 	forall k, k < n -> (rotr n m) k < n.
 Proof.
-	intros. unfold rotr. destruct_if; [lia|].
+	intros. unfold rotr. bdestruct_one; [lia|].
 	apply Nat.mod_upper_bound; lia.
 Qed.
 
 Lemma rotl_bdd {n m} : 
 	forall k, k < n -> (rotl n m) k < n.
 Proof.
-	intros. unfold rotl. destruct_if; [lia|].
+	intros. unfold rotl. bdestruct_one; [lia|].
 	apply Nat.mod_upper_bound; lia.
 Qed.
 
@@ -999,9 +1411,9 @@ Lemma rotr_rotl_inv n m :
 Proof.
 	apply functional_extensionality; intros k.
 	unfold compose, rotl, rotr.
-	bdestruct (n <=? k); [destruct_if_solve|].
+	bdestruct (n <=? k); [bdestructΩ'|].
 	assert (Hn0 : n <> 0) by lia.
-	destruct_if.
+	bdestruct_one.
 	- pose proof (Nat.mod_upper_bound (k + (n - m mod n)) n Hn0) as Hbad.
 	  lia. (* contradict Hbad *)
 	- rewrite Nat.add_mod_idemp_l; [|easy].
@@ -1021,9 +1433,9 @@ Lemma rotl_rotr_inv n m :
 Proof.
 	apply functional_extensionality; intros k.
 	unfold compose, rotl, rotr.
-	bdestruct (n <=? k); [destruct_if_solve|].
+	bdestruct (n <=? k); [bdestructΩ'|].
 	assert (Hn0 : n <> 0) by lia.
-	destruct_if.
+	bdestruct_one.
 	- pose proof (Nat.mod_upper_bound (k + m) n Hn0) as Hbad.
 	  lia. (* contradict Hbad *)
 	- rewrite Nat.add_mod_idemp_l; [|easy].
@@ -1058,7 +1470,7 @@ Lemma rotr_0_r n : rotr n 0 = idn.
 Proof.
 	apply functional_extensionality; intros k.
 	unfold rotr.
-	destruct_if_solve.
+	bdestructΩ'.
 	rewrite Nat.mod_small; lia.
 Qed.
 
@@ -1066,7 +1478,7 @@ Lemma rotl_0_r n : rotl n 0 = idn.
 Proof.
 	apply functional_extensionality; intros k.
 	unfold rotl.
-	destruct_if_solve.
+	bdestructΩ'.
 	rewrite Nat.mod_0_l, Nat.sub_0_r; [|lia].
 	replace (k + n) with (k + 1 * n) by lia.
 	rewrite Nat.mod_add, Nat.mod_small; lia.
@@ -1076,14 +1488,14 @@ Lemma rotr_0_l k : rotr 0 k = idn.
 Proof.
 	apply functional_extensionality; intros a.
 	unfold rotr.
-	destruct_if_solve.
+	bdestructΩ'.
 Qed.
 	
 Lemma rotl_0_l k : rotl 0 k = idn.
 Proof.
 	apply functional_extensionality; intros a.
 	unfold rotl.
-	destruct_if_solve.
+	bdestructΩ'.
 Qed.
 
 #[export] Hint Rewrite rotr_0_r rotl_0_r rotr_0_l rotl_0_l : perm_cleanup_db.
@@ -1094,7 +1506,7 @@ Proof.
 	apply functional_extensionality; intros a.
 	unfold compose, rotr.
 	symmetry.
-	destruct_if_solve; assert (Hn0 : n <> 0) by lia.
+	bdestructΩ'; assert (Hn0 : n <> 0) by lia.
 	- pose proof (Nat.mod_upper_bound (a + l) n Hn0); lia.
 	- rewrite Nat.add_mod_idemp_l; [|easy].
 	  f_equal; lia.
@@ -1118,7 +1530,7 @@ Lemma rotr_n n : rotr n n = idn.
 Proof.
 	apply functional_extensionality; intros a.
 	unfold rotr.
-	destruct_if_solve.
+	bdestructΩ'.
 	replace (a + n) with (a + 1 * n) by lia.
 	destruct n; [lia|].
 	rewrite Nat.mod_add; [|easy].
@@ -1143,14 +1555,14 @@ Qed.
 
 Lemma rotl_n n : rotl n n = idn.
 Proof.
-  by_inverse_injective (rotr n n) n.
+  perm_eq_by_WF_inv_inj (rotr n n) n.
 Qed.
 
 #[export] Hint Rewrite rotl_n : perm_cleanup_db.
 
 Lemma rotl_eq_rotl_mod n k : rotl n k = rotl n (k mod n).
 Proof. 
-  by_inverse_injective (rotr n k) n.
+  perm_eq_by_WF_inv_inj (rotr n k) n.
   rewrite rotr_eq_rotr_mod, rotl_rotr_inv; easy.
 Qed.
 
@@ -1158,7 +1570,7 @@ Lemma rotr_eq_rotl_sub n k :
 	rotr n k = rotl n (n - k mod n).
 Proof.
 	rewrite rotr_eq_rotr_mod.
-  by_inverse_injective (rotl n (k mod n)) n.
+  perm_eq_by_WF_inv_inj (rotl n (k mod n)) n.
   cleanup_perm.
 	destruct n; [rewrite rotl_0_l; easy|].
   assert (H': S n <> 0) by easy.
@@ -1171,7 +1583,7 @@ Qed.
 Lemma rotl_eq_rotr_sub n k : 
 	rotl n k = rotr n (n - k mod n).
 Proof.
-  by_inverse_injective (rotr n k) n.
+  perm_eq_by_WF_inv_inj (rotr n k) n.
 	destruct n; [cbn; rewrite 2!rotr_0_l, compose_idn_l; easy|].
   rewrite (rotr_eq_rotr_mod _ k), rotr_rotr, <- (rotr_n (S n)).
   f_equal.
