src/CategoryTypeclass/DaggerMonoidal.v
@@ -1,11 +1,11 @@
 Require Import CoreData.
 Require Import CoreRules.
+Require Import Permutation.
+Require Import PermutationRules.
 Require Import Category.
 Require Import Dagger.
 Require Import Monoidal.
 Require Import MonoidalRules.
-Require Import Permutation.
-Require Import PermutationRules.
 
 Local Open Scope Cat.
 
