src/Permutations/PermutationAutomation.v
@@ -2,82 +2,84 @@ Require Export CoreData.ZXCore.
 Require Export PermutationDefinitions.
 Require Export QuantumLib.Permutations.
 Require Export CoreRules.CoreAutomation.
+Require Export ZXperm.
 
 (* TODOs: 
     - Declare databases
     - Remove all these random tactics; replace with the standard ones
 *)
 
-Create HintDb WF_Perm_db.
-#[export] Hint Resolve monotonic_WF_Perm compose_WF_Perm : WF_Perm_db.
+Create HintDb perm_db.
+Create HintDb perm_bdd_db.
+Create HintDb perm_inv_db.
+Create HintDb WF_perm_db.
+
+<<<<<<< Updated upstream
+(* Create HintDb perm_cleanup_db.
+Create HintDb perm_of_zx_cleanup_db. *)
+
+Create HintDb zxperm_db.
+#[export] Hint Constructors ZXperm : zxperm_db.
+
+(* TODO: Once quantumlib's up, put these things here: *)
+(* Create HintDb WF_perm_db. *)
+(* #[export] Hint Resolve monotonic_WF_perm compose_WF_perm : WF_perm_db. *)
 
 
-Tactic Notation "tryeasylia" :=
-  try easy; try lia.
+(* Tactic Notation "tryeasylia" :=
+  try easy; try lia. *)
+
+
+
+Ltac replace_bool_lia b0 b1 :=
+  first [
+    replace b0 with b1 by (bdestruct b0; lia || (destruct b1 eqn:?; lia)) |
+    replace b0 with b1 by (bdestruct b1; lia || (destruct b0 eqn:?; lia)) |
+    replace b0 with b1 by (bdestruct b0; bdestruct b1; lia)
+  ].
+=======
+
 
 
 
 Ltac bdest_lia_replace b0 b1 :=
   replace b0 with b1 by (bdestruct b0; lia).
+>>>>>>> Stashed changes
 
 Ltac show_permutation :=
   repeat first [
     split
   | simpl; solve [auto with perm_db]
   | subst; solve [auto with perm_db]
-  | auto with perm_db
   | solve [eauto using permutation_compose with perm_db]
   | easy
   | lia
   ].
 
-Ltac enumerate_value i :=
-  destruct i; [|tryif lia then idtac else enumerate_value i].
 
-Ltac enumerate_matrix Hi Hj :=
-  match type of Hi with (?i < ?n)%nat =>
-  match type of Hj with (?j < ?m)%nat => 
-  enumerate_value i; enumerate_value j
-  (* repeat first [destruct i; destruct j; try lia] *)
-  end end.
 
-  (* by_cell *)
-
-Ltac check_finite_matrix :=
-  apply mat_equiv_eq;
-  try auto with wf_db;
-  intros i j Hi Hj; simpl in *;
-  enumerate_matrix Hi Hj;
-  try lia;
-  try easy.
-
-  (* solve_matrix *)
-
-  
-
-Ltac bdestshoweq := (* goal of form b0 = b1, bools *)
-  match goal with 
-  | |- ?b0 = ?b1 =>
-    bdestruct b0; bdestruct b1; auto; try easy; lia
-  end.
-
-Ltac fail_if_iffy H :=
-  match H with
-  | context[if _ then _ else _] => fail 1
-  | _ => idtac
-  end.
-
-Ltac destruct_if :=
+Ltac bdestruct_one :=
+  let fail_if_iffy H :=
+    match H with
+    | context[if _ then _ else _] => fail 1
+    | _ => idtac
+    end
+  in
   match goal with
-  | [ |- context[if ?b then _ else _]] 
-      => fail_if_iffy b; bdestruct b
+  | |- context [ ?a <? ?b ] => fail_if_iffy a; fail_if_iffy b; bdestruct (a <? b)
+  | |- context [ ?a <=? ?b ] => fail_if_iffy a; fail_if_iffy b; bdestruct (a <=? b)
+  | |- context [ ?a =? ?b ] => fail_if_iffy a; fail_if_iffy b; bdestruct (a =? b)
+  | |- context[if ?b then _ else _]
+      => fail_if_iffy b; destruct b eqn:?
   end.
 
-Ltac destruct_if_solve :=
-  repeat (destruct_if; subst; tryeasylia);
+
+Ltac bdestructΩ' :=
+  let tryeasylia := try easy; try lia in 
+  repeat (bdestruct_one; subst; tryeasylia);
   tryeasylia.
 
-(* From: http://adam.chlipala.net/cpdt/html/Match.html *)
+(* From: http://adam.chlipala.net/cpdt/html/Match.html
 
 Ltac notHyp P :=
   match goal with
@@ -92,19 +94,19 @@ Ltac notHyp P :=
 (* Also from above source *)
 Ltac extend pf :=
   let t := type of pf in
-    notHyp t; generalize pf; intro.
+    notHyp t; generalize pf; intro. *)
 
-Ltac add_mod_bound a n :=
+(* Ltac add_mod_bound a n :=
   let Han := fresh "Han" in assert(Han : a mod n < n)
-    by solve [apply Nat.mod_upper_bound; tryeasylia]; extend (Han).
+    by solve [apply Nat.mod_upper_bound; tryeasylia]; extend (Han). *)
 
-Ltac destruct_if_solve_mods :=
-  repeat (destruct_if; subst; tryeasylia);
+(* Ltac bdestructΩ'_mods :=
+  repeat (bdestruct_one; subst; tryeasylia);
   repeat match goal with
     | [ _ : context[?a mod ?n] |- _] => add_mod_bound a n
     | [ |- context[?a mod ?n]] => add_mod_bound a n
     end;
-  tryeasylia.
+  tryeasylia. *)
 
 
 
@@ -133,6 +135,7 @@ Tactic Notation "cleanup_perm_of_zx" :=
   auto_cast_eqn (autorewrite with perm_of_zx_cleanup_db perm_inv_db perm_cleanup_db). *)
 
 
+
 Tactic Notation "cleanup_perm_inv" := 
   autorewrite with perm_inv_db.
 
@@ -145,11 +148,12 @@ Tactic Notation "cleanup_perm_of_zx" :=
 Lemma compose_id_of_compose_idn {f g : nat -> nat} 
   (H : (f ∘ g)%prg = (fun n => n)) {k : nat} : f (g k) = k.
 Proof.
-  apply_f H k.
+  apply (f_equal_inv k) in H.
   easy.
 Qed.
 
 Ltac perm_by_inverse finv :=
+  let tryeasylia := try easy; try lia in 
   exists finv;
   intros k Hk; repeat split;
   only 3,4 : (try apply compose_id_of_compose_idn; cleanup_perm; tryeasylia) 
@@ -160,24 +164,308 @@ Ltac perm_by_inverse finv :=
 
 
 Ltac solve_stack_perm n0 n1 :=
+  let tryeasylia := try easy; try lia in 
   apply functional_extensionality; intros k;
   unfold stack_perms;
   bdestruct (k <? n0)%nat; [tryeasylia|];
   try bdestruct (k <? n0 + n1)%nat; tryeasylia.
   
 Ltac solve_stack_perm_strong n0 n1 :=
+  let tryeasylia := try easy; try lia in 
   unfold stack_perms; 
   apply functional_extensionality; intros k;
   bdestruct (k <? n0)%nat; [tryeasylia | ]; try bdestruct (k <? n0 + n1);
-  destruct_if_solve.
-(* ^ REPLACED BY: solve_stack_perm; destruct_if_solve *)
+  bdestructΩ'.
+(* ^ REPLACED BY: solve_stack_perm; bdestructΩ' *)
 
 
 (* TODO: Figure out order of operations on where to put this vs its lemma *)
-(* Ltac by_inverse_injective f n :=
+(* Ltac perm_eq_by_WF_inv_inj f n :=
   apply (WF_permutation_inverse_injective f n); [
     tryeasylia; auto with perm_db |
-    tryeasylia; auto with perm_WF_db |
+    tryeasylia; auto with WF_perm_db |
     try solve [cleanup_perm; auto] |
     try solve [cleanup_perm; auto]]; tryeasylia. *)
 
+
+
+
+
+
+Lemma mod_add_n_r : forall m n, 
+	(m + n) mod n = m mod n.
+Proof.
+	intros m n.
+	replace (m + n)%nat with (m + 1 * n)%nat by lia.
+	destruct n.
+	- cbn; easy.
+	- rewrite Nat.mod_add;
+		lia.
+Qed.
+
+Lemma mod_eq_sub : forall m n,
+	m mod n = (m - n * (m / n))%nat.
+Proof.
+	intros m n.
+	destruct n.
+	- cbn; lia.
+	- assert (H: (S n <> 0)%nat) by easy.
+		pose proof (Nat.div_mod m (S n) H) as Heq.
+		lia.
+Qed.
+
+Lemma mod_of_scale : forall m n q, 
+	(n * q <= m < n * S q)%nat -> m mod n = (m - q * n)%nat.
+Proof.
+	intros m n q [Hmq HmSq].
+	rewrite mod_eq_sub.
+	replace (m/n)%nat with q; [lia|].
+	apply Nat.le_antisymm.
+	- apply Nat.div_le_lower_bound; lia. 
+	- epose proof (Nat.div_lt_upper_bound m n (S q) _ _).
+		lia.
+		Unshelve.
+		all: lia.
+Qed.
+
+Lemma mod_n_to_2n : forall m n, 
+	(n <= m < 2 * n)%nat -> m mod n = (m - n)%nat.
+Proof.
+	intros.
+	epose proof (mod_of_scale m n 1 _).
+	lia.
+	Unshelve.
+	lia.
+Qed.
+
+Lemma mod_n_to_n_plus_n : forall m n, 
+	(n <= m < n + n)%nat -> m mod n = (m - n)%nat.
+Proof.
+	intros.
+	apply mod_n_to_2n; lia.
+Qed.
+
+Ltac simplify_mods_of a b :=
+	first [
+		rewrite (Nat.mod_small a b) in * by lia
+	| rewrite (mod_n_to_2n a b) in * by lia
+	].
+
+Ltac solve_simple_mod_eqns :=
+  let __fail_if_has_mods a :=
+    match a with
+    | context[_ mod _] => fail 1
+    | _ => idtac
+    end
+  in
+	match goal with
+	| |- context[if _ then _ else _] => fail 1 "Cannot solve equation with if"
+	| _ =>
+		repeat first [
+      easy
+	  |	lia
+		|	match goal with 
+			| |- context[?a mod ?b] => __fail_if_has_mods a; __fail_if_has_mods b; 
+					simplify_mods_of a b
+			| H: context[?a mod ?b] |- _ => __fail_if_has_mods a; __fail_if_has_mods b; 
+					simplify_mods_of a b
+			end 
+		| match goal with
+			| |- context[?a mod ?b] => (* idtac a b; *) bdestruct (a <? b);
+					[rewrite (Nat.mod_small a b) by lia 
+					| try rewrite (mod_n_to_2n a b) by lia]
+			end
+		]
+	end.
+
+Ltac solve_modular_permutation_equalities :=
+  first [cleanup_perm_of_zx | cleanup_perm_inv | cleanup_perm];
+  unfold Basics.compose, rotr, rotl, stack_perms, swap_perm,
+  (* TODO: remove *) swap_2_perm;
+  apply functional_extensionality; let k := fresh "k" in intros k;
+  bdestructΩ';
+  solve_simple_mod_eqns.
+
+
+
+(* Hack to get auto to apply PermStack where it obviously should 
+  (like to ZXperm (S n) (— ↕ zx), where zx : ZX n n; it doesn't work 
+  here because apply doesn't see that S n = 1 + n, but if we tell it
+  to look for 1 + n, it will find S n). *)
+Ltac __cleanup_stack_perm zx0 zx1 :=
+  match type of zx0 with ZX ?n0 ?n0 =>
+  match type of zx1 with ZX ?n1 ?n1 =>
+  apply (PermStack (n0:=n0) (n1:=n1))
+  end end.
+
+#[export] Hint Extern 0 (ZXperm _ (?zx0 ↕ ?zx1)) => __cleanup_stack_perm zx0 zx1 : zxperm_db.
+
+(* Making proportional_of_eq_perm usable, mostly through a series of tactics to
+   deal with the absolute nightmare that is definitional equality casts. *)
+Lemma prop_iff_double_cast : forall {n0 m0} n1 m1 (zx0 zx1 : ZX n0 m0) 
+  (prfn: n1 = n0) (prfm : m1 = m0),
+  Proportional.proportional zx0 zx1 <-> Proportional.proportional (cast n1 m1 prfn prfm zx0) (cast _ _ prfn prfm zx1).
+Proof.
+    intros.
+    subst.
+    reflexivity.
+Qed.
+
+Ltac __cast_prop_sides_to_square :=
+  match goal with
+  | |- Proportional.proportional ?zx0 ?zx1 =>
+    match type of zx0 with 
+    | ZX ?n ?n => idtac
+    | ZX ?n ?m => 
+      let Hm0n := fresh "Hm0n" in 
+      assert (Hm0n : n = m) by lia;
+      rewrite (prop_iff_double_cast n n zx0 zx1 (eq_refl) (Hm0n))
+    end
+  end.
+
+Lemma cast_compose_eq : forall n0 n1 m o0 o1 (zx0 : ZX n0 m) (zx1 : ZX m o0) Hn0n1 Ho0o1,
+  cast n1 o1 Hn0n1 Ho0o1 (zx0 ⟷ zx1) = 
+  (cast n1 m Hn0n1 (@eq_refl _ m) zx0) ⟷ (cast m o1 (@eq_refl _ m) Ho0o1 zx1).
+Proof.
+  intros.
+  subst.
+  reflexivity.
+Qed.
+
+Lemma cast_cast_eq : forall n0 m0 n1 m1 n2 m2 (zx : ZX n0 m0) Hn0n1 Hm0m1 Hn1n2 Hm1m2,
+  let Hn0n2 := eq_trans Hn1n2 Hn0n1 in
+  let Hm0m2 := eq_trans Hm1m2 Hm0m1 in
+  cast n2 m2 Hn1n2 Hm1m2 (cast n1 m1 Hn0n1 Hm0m1 zx) =
+  cast n2 m2 Hn0n2 Hm0m2 zx.
+Proof.
+  intros; subst.
+  reflexivity.
+Qed.
+
+Section Isolated.
+(* TODO: This is really ugly. Can I get around it? *)
+(* Note these next two lemmas are subsumed by the third, but I'm keeping them
+   to exemplify how weird doing this is... *)
+Lemma nat_equality_proof_equality : forall (n m : nat) (H0 H1 : n = m),
+  H0 = H1.
+Proof.
+  intros n. intros.
+  subst n.
+  now rewrite Logic.Eqdep_dec.UIP_refl_nat.
+Qed.
+
+Lemma cast_proof_independence : forall n0 m0 n1 m1 (zx : ZX n0 m0) prfn1 prfm1 prfn2 prfm2,
+  cast n1 m1 prfn1 prfm1 zx = cast n1 m1 prfn2 prfm2 zx.
+Proof.
+  intros. 
+  (* Logic.Eqdep_dec.UIP_refl_nat *)
+  (* Search "extensionality". *)
+  replace prfn2 with prfn1 by (apply nat_equality_proof_equality).
+  replace prfm2 with prfm1 by (apply nat_equality_proof_equality).
+  reflexivity.
+Qed.
+End Isolated.
+
+(* Also, note that this doesn't introduce any new axioms. It's just __weird__. *)
+(* Print Assumptions Eqdep_dec.UIP_refl_nat. ("Closed under the global context")*)
+
+Lemma cast_id_eq : forall n m (prfn : n = n) (prfm : m = m) zx,
+  cast n m prfn prfm zx = zx.
+Proof.
+  intros; subst.
+  rewrite (Eqdep_dec.UIP_refl_nat n prfn). (* Replace prfn with (@eq_refl nat n) *)
+  rewrite (Eqdep_dec.UIP_refl_nat m prfm). (* Replace prfn with (@eq_refl nat m) *)
+  reflexivity.
+Qed.
+
+Lemma zxperm_iff_cast' : forall n0 n1 zx (H H' : n1 = n0),
+  ZXperm n1 (cast n1 n1 H H' zx) <-> ZXperm n0 zx.
+Proof.
+  intros.
+  subst; rewrite cast_id_eq.
+  reflexivity.
+Qed.
+
+#[export] Hint Resolve <- zxperm_iff_cast' : zxperm_db.
+
+Ltac simpl_permlike_zx :=
+  let simpl_casts_eq := first [
+    rewrite cast_id_eq |
+    rewrite cast_cast_eq ]
+  in
+  repeat (match goal with
+  | |- context[?zx ⟷ cast ?m' ?o' ?prfm ?prfo (n_wire ?o)] =>
+    rewrite (@CastRules.cast_compose_r _ _ _ _ _ prfm prfo zx _);
+    rewrite (@ComposeRules.nwire_removal_r o)
+  | |- context[cast ?n' ?m' ?prfn ?prfm (n_wire ?n) ⟷ ?zx] => idtac "match";
+    rewrite (@CastRules.cast_compose_l _ _ _ _ _ prfn prfm _ zx);
+    rewrite (@ComposeRules.nwire_removal_l n)
+  | |- context[@cast ?n' ?m' ?n ?m ?prfn ?prfm ?zx ⟷ cast ?m' ?o' ?prfom ?prfo (n_wire ?o)] =>
+    rewrite (@CastRules.cast_compose_l n n' m m' o' prfn prfm zx (cast m' o' prfom prfo (n_wire o)));
+    rewrite (cast_cast_eq _ _ _ _ _ _ (n_wire o));
+    try rewrite (cast_id_eq _ _ _ _ (zx ⟷ _))
+  | |- context[cast ?n ?m' ?prfn ?prfmn (n_wire ?n') ⟷ @cast ?m' ?o' ?m ?o ?prfm ?prfo ?zx] =>
+    rewrite (@CastRules.cast_compose_r n m m' o o' prfm prfo (cast n m prfn prfmn (n_wire n')) zx);
+    rewrite (cast_cast_eq _ _ _ _ _ _ (n_wire n'));
+    try rewrite (cast_id_eq _ _ _ _ (zx ⟷ _))
+  | |- context[cast ?n1 ?m _ _ ?zx0 ⟷ cast ?m ?o1 _ _ ?zx1] =>
+    rewrite <- (cast_compose_eq _ n1 m _ o1 zx0 zx1)
+  | |- context[ @cast ?n1 ?m1 ?n0 ?m0 ?prfn0 ?prfm0 ?zx0 ⟷ cast ?m1 ?o1 ?prfm1 ?prfo1 ?zx1 ] => idtac "match";
+    rewrite (CastRules.cast_compose_mid m0 (eq_sym prfm0) (eq_sym prfm0) (cast n1 m1 prfn0 prfm0 zx0) (cast m1 o1 prfm1 prfo1 zx1));
+    rewrite
+      (cast_cast_eq _ _ _ _ _ _ zx0), (cast_cast_eq _ _ _ _ _ _ zx1),
+      (cast_id_eq _ _ _ _ zx0)
+end; repeat simpl_casts_eq).
+
+
+
+#[export] Hint Extern 2 => (repeat first [rewrite cast_id_eq | rewrite cast_cast_eq]) : zxperm_db.
+
+Ltac __one_round_cleanup_zxperm_of_cast :=
+  match goal with
+  | |- ZXperm _ (cast ?n2 ?m2 ?Hn1n2 ?Hm1m2 (@cast ?n1 ?m1 ?n0 ?m0 ?Hn0n1 ?Hm0m1 ?zx)) => (* idtac "clean_cast_cast"; *)
+    rewrite (cast_cast_eq n0 m0 n1 m1 n2 m2 zx Hn0n1 Hm0m1 Hn1n2 Hm1m2)
+  | |- ZXperm ?n (@cast ?n ?n ?n ?n _ _ ?zx) => (* idtac "clean_id";  *)
+    rewrite (cast_id_eq n n _ _ zx)
+  | |- ZXperm ?n (@cast ?n ?n ?n' ?m' _ _ (?zx0 ⟷ ?zx1)) => (* idtac "clean_comp"; *)
+    rewrite (cast_compose_eq _ _ _ _ _ zx0 zx1) by lia; 
+    apply PermComp
+  | |- ZXperm ?n (@cast ?n ?n ?n' ?m' _ _ (?zx0 ↕ ?zx1)) => (* idtac "clean_stack"; *)
+    match type of zx0 with ZX ?n0 ?n0 =>
+    match type of zx1 with ZX ?n1 ?n1 =>
+      rewrite <- (zxperm_iff_cast' (n) (n0 + n1) (ltac:(lia)) (ltac:(lia)))
+    end end
+  end.
+
+#[export] Hint Extern 3 (ZXperm _ (cast _ _ _ _ _)) => __one_round_cleanup_zxperm_of_cast : zxperm_db.
+
+Lemma perm_of_cast_compose_each_square : forall n m a b c d
+  (zx0 : ZX n n) (zx1 : ZX m m) prfa0 prfb0 prfb1 prfc1 prfd1 prfd2,
+  ZXperm n zx0 -> ZXperm m zx1 ->
+  ZXperm d (cast d d prfd1 prfd2 
+  (cast a b prfa0 prfb0 zx0 ⟷ cast b c prfb1 prfc1 zx1)).
+Proof.
+  intros.
+  subst.
+  auto with zxperm_db.
+Qed.
+
+#[export] Hint Resolve perm_of_cast_compose_each_square : zxperm_db.
+
+(* This can't be here because proportional_of_eq_perm is defined later, but keeping 
+   for reference. (This is put in ZXpermSemantics, right after proportional_of_eq_perm.) *)
+
+(*
+Ltac prop_perm_eq :=
+  intros;
+  simpl_casts;
+  simpl_permlike_zx;
+  __cast_prop_sides_to_square;
+  (* Goal: zx0 ∝ zx1 *)
+  apply proportional_of_eq_perm; [
+  (* New goals: *)
+    (*1: ZXperm _ zx0 *) auto with zxperm_db |
+    (*2: ZXperm _ zx1*) auto with zxperm_db |
+    (*3: perm_of_zx zx0 = perm_of_zx zx1*) cleanup_perm_of_zx; try easy; try lia
+  ].
+*)
