src/Permutations/PermutationInstances.v
@@ -34,13 +34,13 @@ Qed.
 
 #[export] Hint Resolve swap_2_perm_bdd : perm_bdd_db.
 
-Lemma swap_2_perm_WF k : 1 < k -> swap_2_perm k = k.
+Lemma swap_2_WF_perm k : 1 < k -> swap_2_perm k = k.
 Proof.
   intros. 
   repeat first [easy | lia | destruct k].
 Qed.
 
-Global Hint Resolve swap_2_perm_WF : perm_WF_db.
+Global Hint Resolve swap_2_WF_perm : WF_perm_db.
 
 Lemma swap_2_perm_permutation : permutation 2 swap_2_perm.
 Proof. 
@@ -63,7 +63,7 @@ Lemma stack_perms_WF_idn {n0 n1} {f}
 	(H : forall k, n0 <= k -> f k = k): 
 	stack_perms n0 n1 f idn = f.
 Proof.
-	solve_stack_perm n0 n1;
+	solve_modular_permutation_equalities;
 	rewrite H; lia.
 Qed.
 
@@ -72,10 +72,10 @@ Lemma stack_perms_WF {n0 n1} {f g} k :
 Proof.
   intros H.
   unfold stack_perms.
-  destruct_if_solve.
+  bdestructΩ'.
 Qed.
 
-Global Hint Resolve stack_perms_WF : perm_WF_db.
+Global Hint Resolve stack_perms_WF : WF_perm_db.
 
 Lemma stack_perms_bdd {n0 n1} {f g}
   (Hf : forall k, k < n0 -> f k < n0) (Hg : forall k, k < n1 -> g k < n1) :
@@ -98,7 +98,7 @@ Lemma stack_perms_rinv {n0 n1} {f g} {finv ginv}
   stack_perms n0 n1 f g ∘ stack_perms n0 n1 finv ginv = idn.
 Proof.
   unfold compose.
-  solve_stack_perm_strong n0 n1.
+  solve_modular_permutation_equalities.
   1-3: specialize (Hf _ H); lia.
   - replace (ginv (k - n0) + n0 - n0) with (ginv (k - n0)) by lia.
     assert (Hkn0: k - n0 < n1) by lia.
@@ -146,25 +146,25 @@ Global Hint Resolve stack_perms_permutation : perm_db.
 (* Section on rotr/rotl *)
 (* Lemma rotr_WF {n m} : 
 	forall k, n <= k -> (rotr n m) k = k.
-Proof. intros. unfold rotr. destruct_if; lia. Qed.
+Proof. intros. unfold rotr. bdestruct_one; lia. Qed.
 
 Lemma rotl_WF {n m} : 
 	forall k, n <= k -> (rotl n m) k = k.
-Proof. intros. unfold rotl. destruct_if; lia. Qed.
+Proof. intros. unfold rotl. bdestruct_one; lia. Qed.
 
-Global Hint Resolve rotr_WF rotl_WF : perm_WF_db.
+Global Hint Resolve rotr_WF rotl_WF : WF_perm_db.
 
 Lemma rotr_bdd {n m} : 
 	forall k, k < n -> (rotr n m) k < n.
 Proof.
-	intros. unfold rotr. destruct_if; [lia|].
+	intros. unfold rotr. bdestruct_one; [lia|].
 	apply Nat.mod_upper_bound; lia.
 Qed.
 
 Lemma rotl_bdd {n m} : 
 	forall k, k < n -> (rotl n m) k < n.
 Proof.
-	intros. unfold rotl. destruct_if; [lia|].
+	intros. unfold rotl. bdestruct_one; [lia|].
 	apply Nat.mod_upper_bound; lia.
 Qed.
 
@@ -175,9 +175,9 @@ Lemma rotr_rotl_inv n m :
 Proof.
 	apply functional_extensionality; intros k.
 	unfold compose, rotl, rotr.
-	bdestruct (n <=? k); [destruct_if_solve|].
+	bdestruct (n <=? k); [bdestructΩ'|].
 	assert (Hn0 : n <> 0) by lia.
-	destruct_if.
+	bdestruct_one.
 	- pose proof (Nat.mod_upper_bound (k + (n - m mod n)) n Hn0) as Hbad.
 	  lia. (* contradict Hbad *)
 	- rewrite Nat.add_mod_idemp_l; [|easy].
@@ -197,9 +197,9 @@ Lemma rotl_rotr_inv n m :
 Proof.
 	apply functional_extensionality; intros k.
 	unfold compose, rotl, rotr.
-	bdestruct (n <=? k); [destruct_if_solve|].
+	bdestruct (n <=? k); [bdestructΩ'|].
 	assert (Hn0 : n <> 0) by lia.
-	destruct_if.
+	bdestruct_one.
 	- pose proof (Nat.mod_upper_bound (k + m) n Hn0) as Hbad.
 	  lia. (* contradict Hbad *)
 	- rewrite Nat.add_mod_idemp_l; [|easy].
@@ -250,7 +250,7 @@ Lemma bottom_to_top_perm_bdd {n} k :
 Proof.
 	intros Hk.
 	unfold bottom_to_top_perm.
-	bdest_lia_replace (n <=? k) false.
+	replace_bool_lia (n <=? k) false.
 	destruct k; lia.
 Qed.
 
@@ -259,31 +259,31 @@ Lemma top_to_bottom_perm_bdd {n} k :
 Proof.
 	intros Hk.
 	unfold top_to_bottom_perm.
-	bdest_lia_replace (n <=? k) false.
+	replace_bool_lia (n <=? k) false.
 	bdestruct (k =? n - 1); lia.
 Qed.
 
 Global Hint Resolve bottom_to_top_perm_bdd top_to_bottom_perm_bdd : perm_bdd_db.
 
-Lemma bottom_to_top_perm_WF {n} k : n <= k ->
+Lemma bottom_to_top_WF_perm {n} k : n <= k ->
 	bottom_to_top_perm n k = k.
 Proof.
 	intros Hk.
 	unfold bottom_to_top_perm.
-	bdest_lia_replace (n <=? k) true.
+	replace_bool_lia (n <=? k) true.
 	easy.
 Qed.
 
-Lemma top_to_bottom_perm_WF {n} k : n <= k ->
+Lemma top_to_bottom_WF_perm {n} k : n <= k ->
 	top_to_bottom_perm n k = k.
 Proof.
 	intros Hk.
 	unfold top_to_bottom_perm.
-	bdest_lia_replace (n <=? k) true.
+	replace_bool_lia (n <=? k) true.
 	easy.
 Qed.
 	
-Global Hint Resolve bottom_to_top_perm_WF top_to_bottom_perm_WF : perm_WF_db.
+Global Hint Resolve bottom_to_top_WF_perm top_to_bottom_WF_perm : WF_perm_db.
 
 Lemma bottom_to_top_to_bottom_inv n : 
 	bottom_to_top_perm n ∘ top_to_bottom_perm n = idn.
@@ -291,13 +291,13 @@ Proof.
 	apply functional_extensionality; intros k.
 	unfold compose, bottom_to_top_perm, top_to_bottom_perm.
 	bdestruct (n <=? k).
-	1: bdest_lia_replace (n <=? k) true; easy.
+	1: replace_bool_lia (n <=? k) true; easy.
 	bdestruct (k =? n - 1).
 	- destruct n.
 	  + easy.
-	  + bdest_lia_replace (S n <=? 0) false.
+	  + replace_bool_lia (S n <=? 0) false.
 	  	lia.
-	- bdest_lia_replace (n <=? k + 1) false.
+	- replace_bool_lia (n <=? k + 1) false.
 	  replace (k + 1) with (S k) by lia.
 	  easy.
 Qed.
@@ -308,14 +308,14 @@ Proof.
 	apply functional_extensionality; intros k.
 	unfold compose, bottom_to_top_perm, top_to_bottom_perm.
 	bdestruct (n <=? k).
-	1: bdest_lia_replace (n <=? k) true; easy.
+	1: replace_bool_lia (n <=? k) true; easy.
 	destruct k.
 	- destruct n; [easy|].
-	  bdest_lia_replace (S n <=? S n - 1) false.
+	  replace_bool_lia (S n <=? S n - 1) false.
 	  rewrite Nat.eqb_refl.
 	  easy.
-	- bdest_lia_replace (n <=? k) false.
-	  bdest_lia_replace (k =? n - 1) false.
+	- replace_bool_lia (n <=? k) false.
+	  replace_bool_lia (k =? n - 1) false.
 	  lia.
 Qed.
 
@@ -365,7 +365,7 @@ Lemma top_to_bottom_perm_eq_rotr n :
 Proof.
 	apply functional_extensionality; intros k.
 	unfold top_to_bottom_perm, rotr.
-	destruct_if_solve.
+	bdestructΩ'.
 	- subst. 
 	  replace (n - 1 + 1) with n by lia.
 	  rewrite Nat.mod_same; lia.
@@ -377,7 +377,7 @@ Qed.
 Lemma bottom_to_top_perm_eq_rotl n :
 	bottom_to_top_perm n = rotl n 1.
 Proof.
-  by_inverse_injective (top_to_bottom_perm n) n.
+  perm_eq_by_WF_inv_inj (top_to_bottom_perm n) n.
 Qed.
 
 #[export] Hint Rewrite bottom_to_top_perm_eq_rotl : perm_cleanup_db.
