src/Permutations/ZXpermFacts.v
@@ -16,37 +16,37 @@ Require Export PermutationInstances.
 
 Local Open Scope nat.
 
-Lemma zxperm_iff_cast {n0 n1 m0 m1} {zx} (Hn : n1 = n0) (Hm : m1 = m0) :
-	ZXperm n1 m1 (cast _ _ Hn Hm zx) <-> ZXperm n0 m0 zx.
+Lemma zxperm_iff_cast {n0 n1} {zx} (Hn : n1 = n0) :
+	ZXperm n1 (cast _ _ Hn Hn zx) <-> ZXperm n0 zx.
 Proof.
 	split; intros; subst; easy.
 Qed.
 
-Global Hint Resolve <- zxperm_iff_cast : zxperm_db.
+#[export] Hint Resolve <- zxperm_iff_cast : zxperm_db.
 
-Lemma cast_stack_zxperm {n0 n1 m0 m1 o p} {zx0} {zx1}
-	(H0 : ZXperm n0 m0 zx0) (H1 : ZXperm n1 m1 zx1) 
-	(Hn : o = n0 + n1) (Hm : p = m0 + m1) :
-	ZXperm o p (cast _ _ Hn Hm (zx0 ↕ zx1)).
+Lemma cast_stack_zxperm {n0 n1 o} {zx0} {zx1}
+	(H0 : ZXperm n0 zx0) (H1 : ZXperm n1 zx1) 
+	(Hn : o = n0 + n1) :
+	ZXperm o (cast _ _ Hn Hn (zx0 ↕ zx1)).
 Proof.
   auto with zxperm_db.
 Qed.
 
-Global Hint Resolve cast_stack_zxperm : zxperm_db.
+#[export] Hint Resolve cast_stack_zxperm : zxperm_db.
 
-Lemma transpose_zxperm {n m} {zx} (H : ZXperm n m zx) :
-	ZXperm m n (zx ⊤).
+Lemma transpose_zxperm {n} {zx} (H : ZXperm n zx) :
+	ZXperm n (zx ⊤).
 Proof.
-	induction H; simpl; constructor; try easy.
+	induction H; simpl; constructor; easy.
 Qed.
 
-Global Hint Resolve transpose_zxperm : zxperm_db.
+#[export] Hint Resolve transpose_zxperm : zxperm_db.
 
 
 
 (* Section on core ZXperms *)
 Lemma n_wire_zxperm {n} : 
-	ZXperm n n (n_wire n).
+	ZXperm n (n_wire n).
 Proof.
 	induction n.
 	- constructor.
@@ -54,21 +54,21 @@ Proof.
     apply (PermStack PermWire IHn).
 Qed.
 
-Global Hint Resolve n_wire_zxperm : zxperm_db.
+#[export] Hint Resolve n_wire_zxperm : zxperm_db.
 
-Lemma n_compose_zxperm {n} {zx} (H : ZXperm n n zx) k :
-	ZXperm _ _ (n_compose k zx).
+Lemma n_compose_zxperm {n} {zx} (H : ZXperm n zx) k :
+	ZXperm _ (n_compose k zx).
 Proof.
 	induction k; simpl; auto with zxperm_db.
 Qed.
 
-Global Hint Resolve n_compose_zxperm : zxperm_db.
+#[export] Hint Resolve n_compose_zxperm : zxperm_db.
 
 
 
 (* Section on specific ZXperms *)
 Lemma top_to_bottom_helper_zxperm n :
-	ZXperm (S n) (S n) (top_to_bottom_helper n).
+	ZXperm (S n) (top_to_bottom_helper n).
 Proof.
 	induction n.
 	- constructor.
@@ -78,21 +78,24 @@ Proof.
 	  + apply (PermStack PermWire IHn).
 Qed.
 
-Global Hint Resolve top_to_bottom_helper_zxperm : zxperm_db.
+#[export] Hint Resolve top_to_bottom_helper_zxperm : zxperm_db.
 
 Lemma top_to_bottom_zxperm {n} :
-	ZXperm n n (top_to_bottom n).
+	ZXperm n (top_to_bottom n).
 Proof.
 	destruct n; simpl; auto with zxperm_db.
 Qed.
 
 Lemma bottom_to_top_zxperm {n} :
-	ZXperm n n (bottom_to_top n).
+	ZXperm n (bottom_to_top n).
 Proof.
 	apply transpose_zxperm.
 	apply top_to_bottom_zxperm.
 Qed.
 
+<<<<<<< Updated upstream
+#[export] Hint Resolve top_to_bottom_zxperm bottom_to_top_zxperm : zxperm_db.
+=======
 Global Hint Resolve top_to_bottom_zxperm bottom_to_top_zxperm : zxperm_db.
 
 (* FIXME: Temporary for working only *)
@@ -111,8 +114,15 @@ Qed.
 
 
 
+>>>>>>> Stashed changes
 
+Lemma a_swap_zxperm n : 
+	ZXperm n (a_swap n).
+Proof.
+	induction n; simpl; auto with zxperm_db.
+Qed.
 
+#[export] Hint Resolve a_swap_zxperm : zxperm_db.
 
 
 
@@ -121,8 +131,8 @@ Qed.
 
 
 (* Section on rules for perm_of_zx *)
-Lemma perm_of_zx_WF {n m} {zx} (H : ZXperm n m zx) : forall k, 
-	n <= k -> (perm_of_zx zx) k = k.
+Lemma perm_of_zx_WF {n} {zx} (H : ZXperm n zx) : 
+	WF_perm n (perm_of_zx zx).
 Proof.
 	induction H; intros k Hk; try easy.
 	- simpl.
@@ -131,27 +141,26 @@ Proof.
 	  rewrite stack_perms_high; easy.
 	- simpl.
 	  unfold compose.
-	  pose proof (zxperm_square H).
 	  rewrite IHZXperm1; rewrite IHZXperm2; lia.
-	Qed.
+Qed.
 
-Global Hint Resolve perm_of_zx_WF : perm_WF_db.
+#[export] Hint Resolve perm_of_zx_WF : WF_perm_db.
 
-Lemma stack_perms_zx_idn {n0 m0 n1} {zx} (H : ZXperm n0 m0 zx) :
+Lemma stack_perms_zx_idn {n0 n1} {zx} (H : ZXperm n0 zx) :
 	stack_perms n0 n1 (perm_of_zx zx) idn = 
 	perm_of_zx zx.
 Proof.
 	apply stack_perms_WF_idn.
-  auto with perm_WF_db.
+  auto with WF_perm_db.
 Qed.
 
-#[export] Hint Rewrite @stack_perms_zx_idn : perm_of_zx_cleanup_db.
+#[export] Hint Rewrite @stack_perms_zx_idn using (auto with zxperm_db) : perm_of_zx_cleanup_db.
 
-Lemma stack_perms_idn_zx {n0 n1 m1} {zx} (H : ZXperm n1 m1 zx) :
+Lemma stack_perms_idn_zx {n0 n1} {zx} (H : ZXperm n1 zx) :
 	stack_perms n0 n1 idn (perm_of_zx zx) = 
 	fun k => if k <? n0 then k else (perm_of_zx zx (k - n0)) + n0.
 Proof.
-	solve_stack_perm n0 n1.
+	solve_modular_permutation_equalities.
 	rewrite perm_of_zx_WF; [lia|easy|lia].
 Qed.
 
@@ -175,19 +184,16 @@ Proof. subst. easy. Qed.
   @perm_of_zx_stack_spec
   @perm_of_zx_cast : perm_of_zx_cleanup_db.
 
-Lemma perm_of_transpose_is_rinv {n m} {zx} (H : ZXperm n m zx) :
+Lemma perm_of_transpose_is_rinv {n} {zx} (H : ZXperm n zx) :
 	(perm_of_zx zx ∘ perm_of_zx zx⊤)%prg = idn.
 Proof.
 	rewrite <- perm_of_zx_compose_spec.
 	induction H; apply functional_extensionality; intros k; try easy.
 	- cbn. 
 	  destruct k; [easy|destruct k; [easy|]].
-	  rewrite swap_2_perm_WF; rewrite swap_2_perm_WF; lia.
+	  rewrite swap_2_WF_perm; rewrite swap_2_WF_perm; lia.
 	- simpl.
-    pose proof (zxperm_square H).
-    pose proof (zxperm_square H0).
-    subst.
-	  rewrite stack_perms_compose.
+    rewrite stack_perms_compose.
 	  2,3: auto with perm_db zxperm_db.
 	  rewrite <- 2!perm_of_zx_compose_spec.
 	  rewrite IHZXperm1, IHZXperm2; cleanup_perm.
@@ -201,7 +207,7 @@ Proof.
 	  easy.
 Qed.
 
-Lemma perm_of_transpose_is_linv {n m} {zx} (H : ZXperm n m zx) :
+Lemma perm_of_transpose_is_linv {n} {zx} (H : ZXperm n zx) :
 	(perm_of_zx zx⊤ ∘ perm_of_zx zx)%prg = idn.
 Proof.
 	pose proof (perm_of_transpose_is_rinv (transpose_zxperm H)) as Hinv.
@@ -211,7 +217,7 @@ Qed.
 
 #[export] Hint Rewrite 
   @perm_of_transpose_is_rinv 
-  @perm_of_transpose_is_linv : perm_of_zx_cleanup_db.
+  @perm_of_transpose_is_linv using (auto with zxperm_db) : perm_of_zx_cleanup_db.
 
 
 
@@ -230,7 +236,7 @@ Qed.
 
 #[export] Hint Rewrite perm_of_n_wire : perm_of_zx_cleanup_db.
 
-Lemma perm_of_zx_stack_n_wire {n0 m0} {zx} (H : ZXperm n0 m0 zx) {n1} :
+Lemma perm_of_zx_stack_n_wire {n0} {zx} (H : ZXperm n0 zx) {n1} :
 	perm_of_zx (zx ↕ (n_wire n1)) = perm_of_zx zx.
 Proof.
 	simpl.
@@ -239,7 +245,7 @@ Proof.
 	easy. 
 Qed.
 
-#[export] Hint Rewrite @perm_of_zx_stack_n_wire : perm_of_zx_cleanup_db.
+#[export] Hint Rewrite @perm_of_zx_stack_n_wire using (auto with zxperm_db) : perm_of_zx_cleanup_db.
 
 Lemma perm_of_top_to_bottom_helper_eq {n} :
 	perm_of_zx (top_to_bottom_helper n) = top_to_bottom_perm (S n).
@@ -249,7 +255,7 @@ Proof.
 	destruct n; [destruct k; easy|].
 	simpl.
 	rewrite perm_of_n_wire.
-	rewrite stack_perms_WF_idn; [|apply swap_2_perm_WF].
+	rewrite stack_perms_WF_idn; [|apply swap_2_WF_perm].
 	rewrite stack_perms_idn_zx; [|apply top_to_bottom_helper_zxperm].
 	rewrite H; [|auto].
 	unfold compose.
@@ -259,16 +265,16 @@ Proof.
 	  1: destruct k; [easy|];
 	     destruct k; [easy|];
 		   cbn; destruct (k + 1) eqn:e; 
-       unfold swap_2_perm; destruct_if_solve.
+       unfold swap_2_perm; bdestructΩ'.
 	  destruct k; [lia|].
 	  replace (S k - 1) with k by lia.
 	  unfold top_to_bottom_perm.
-	  replace (S (S (S n)) <=? S k) with (S (S n) <=? k) by bdestshoweq.
-	  replace (S k =? S (S (S n)) - 1) with (k =? S (S n) - 1) by bdestshoweq.
+	  replace_bool_lia (S (S (S n)) <=? S k) (S (S n) <=? k).
+	  replace_bool_lia (S k =? S (S (S n)) - 1) (k =? S (S n) - 1).
 	  bdestruct (S (S n) <=? k).
-	  + rewrite swap_2_perm_WF; lia.
+	  + rewrite swap_2_WF_perm; lia.
 	  + bdestruct (k =? S (S n) - 1); [easy|].
-	    rewrite swap_2_perm_WF; lia.
+	    rewrite swap_2_WF_perm; lia.
 Qed.
 
 #[export] Hint Rewrite @perm_of_top_to_bottom_helper_eq : perm_of_zx_cleanup_db.
@@ -289,7 +295,7 @@ Qed.
 Lemma perm_of_bottom_to_top_eq n :
 	perm_of_zx (bottom_to_top n) = bottom_to_top_perm n.
 Proof.
-  by_inverse_injective (top_to_bottom_perm n) n.
+  perm_eq_by_WF_inv_inj (top_to_bottom_perm n) n.
   rewrite <- perm_of_top_to_bottom_eq.
 	unfold bottom_to_top.
   apply perm_of_transpose_is_linv; auto with zxperm_db.
@@ -337,6 +343,20 @@ Qed.
 
 #[export] Hint Rewrite perm_of_n_compose_n_top_to_bottom : perm_of_zx_cleanup_db.
 
+<<<<<<< Updated upstream
+<<<<<<< Updated upstream
+Lemma perm_of_a_swap n : 
+	perm_of_zx (a_swap n) = swap_perm 0 (n - 1) n.
+Proof.
+	destruct n; [cleanup_perm; easy|].
+	simpl.
+	solve_modular_permutation_equalities.
+Qed.
+
+#[export] Hint Rewrite perm_of_a_swap : perm_of_zx_cleanup_db.
+=======
+=======
+>>>>>>> Stashed changes
 
 
 (* FIXME: This doesn't go here: *)
@@ -472,5 +492,9 @@ Proof.
 		bdestruct_all; solve_simple_mod_eqns.
 Qed.
 
+<<<<<<< Updated upstream
+>>>>>>> Stashed changes
+=======
+>>>>>>> Stashed changes
 
 Local Close Scope nat.
